06GroupedEnvironments/VariableSplitting.thy
@@ -7,7 +7,7 @@ section \<open>Variable splitting\<close>
 text \<open>Now we divide our variables into frame-offset pairs. The process is quite simple for 
 expressions: we accumulate a map from Debruijn indices to frame-offset pairs, adding to it every 
 time we pass a binder, and then map variables when we reach them. (As mentioned before, we also 
-record the frame-size every time we reach a \<open>Lam\<^sub>d\<close>.\<close>
+record the frame-size every time we reach a \<open>Lam\<^sub>d\<close>.)\<close>
 
 abbreviation map_past_lam :: "(nat \<rightharpoonup> nat \<times> nat) \<Rightarrow> nat \<rightharpoonup> nat \<times> nat" where
   "map_past_lam \<Phi> x \<equiv> (case x of 
@@ -28,6 +28,86 @@ primrec split_vars' :: "(nat \<rightharpoonup> nat \<times> nat) \<Rightarrow> e
 
 definition split_vars :: "expr\<^sub>d \<Rightarrow> expr\<^sub>g" where
   "split_vars e \<equiv> split_vars' Map.empty e"
+
+text \<open>With the help of an auxiliary function to generate the splitting map from an environment, we
+can prove type-safety as well.\<close>
+
+fun inv_map_from_env :: "'a list list \<Rightarrow> nat \<rightharpoonup> nat \<times> nat" where
+  "inv_map_from_env [] x = None"
+| "inv_map_from_env (bs # bss) x = (
+    if x < length bs then Some (0, x) 
+    else map_option (apfst Suc) (inv_map_from_env bss (x - length bs)))"
+
+lemma inv_map_from_env_empty [simp]: "inv_map_from_env [] = Map.empty"
+  by auto
+
+lemma inv_map_from_env_insert [simp]: "inv_map_from_env (insert_at 0 [a] as) = 
+    map_past_lam (inv_map_from_env as)"
+  by (induction as) (auto split: nat.splits)
+
+lemma inv_map_from_env_cons_fst [simp]: "inv_map_from_env (cons_fst a as) = 
+    map_past_let (inv_map_from_env as)"
+proof (cases as)
+  case (Cons bs bss)
+
+  have "\<And>x. inv_map_from_env (cons_fst a (bs # bss)) x = 
+    map_past_let (inv_map_from_env (bs # bss)) x" 
+  proof -
+    fix x
+    show "inv_map_from_env (cons_fst a (bs # bss)) x = map_past_let (inv_map_from_env (bs # bss)) x"
+    proof (cases "x > length bs")
+      case True
+      hence "\<exists>k. x = length bs + Suc k" by presburger
+      then obtain k where K: "x = length bs + Suc k" by presburger
+      with True show ?thesis by (simp add: option.map_comp)
+    qed (simp_all split: nat.splits)
+  qed
+  with Cons show ?thesis by auto
+qed (auto split: nat.splits)
+
+lemma lookup_inv_map [simp]: "lookup (concat \<Gamma>) x = Some t \<Longrightarrow> 
+  \<exists>y z ts. inv_map_from_env \<Gamma> x = Some (y, z) \<and> lookup \<Gamma> y = Some ts \<and> lookup ts z = Some t"
+proof (induction \<Gamma> arbitrary: x)
+  case (Cons ts \<Gamma>)
+  thus ?case
+  proof (cases "x < length ts")
+    case False
+    hence "\<exists>k. x = length ts + k" by presburger
+    then obtain k where K: "x = length ts + k" by auto
+    with Cons obtain y z ts' where "inv_map_from_env \<Gamma> k = Some (y, z) \<and> lookup \<Gamma> y = Some ts' \<and> 
+      lookup ts' z = Some t" by fastforce
+    with False K show ?thesis by auto
+  qed auto
+qed simp_all
+
+lemma typecheck_split' [simp]: "concat \<Gamma> \<turnstile>\<^sub>d e : t \<Longrightarrow> \<Gamma> \<turnstile>\<^sub>g split_vars' (inv_map_from_env \<Gamma>) e : t"
+proof (induction "concat \<Gamma>" e t arbitrary: \<Gamma> rule: typing\<^sub>d.induct)
+  case (tc\<^sub>d_var x t)
+  hence "lookup (concat \<Gamma>) x = Some t" by simp
+  then obtain y z ts where "inv_map_from_env \<Gamma> x = Some (y, z) \<and> lookup \<Gamma> y = Some ts \<and> 
+    lookup ts z = Some t" by (metis lookup_inv_map)
+  thus ?case by simp
+next
+  case (tc\<^sub>d_lam t\<^sub>1 e t\<^sub>2)
+  have "insert_at 0 t\<^sub>1 (concat \<Gamma>) = concat (insert_at 0 [t\<^sub>1] \<Gamma>)" by simp
+  with tc\<^sub>d_lam have "insert_at 0 [t\<^sub>1] \<Gamma> \<turnstile>\<^sub>g 
+    split_vars' (inv_map_from_env (insert_at 0 [t\<^sub>1] \<Gamma>)) e : t\<^sub>2" by blast
+  thus ?case by (simp add: Let_def)
+next
+  case (tc\<^sub>d_let e\<^sub>1 t\<^sub>1 e\<^sub>2 t\<^sub>2)
+  have "insert_at 0 t\<^sub>1 (concat \<Gamma>) = concat (cons_fst t\<^sub>1 \<Gamma>)" by simp
+  with tc\<^sub>d_let have "cons_fst t\<^sub>1 \<Gamma> \<turnstile>\<^sub>g split_vars' (inv_map_from_env (cons_fst t\<^sub>1 \<Gamma>)) e\<^sub>2 : t\<^sub>2" 
+    by blast
+  with tc\<^sub>d_let show ?case by fastforce
+qed fastforce+
+
+lemma typecheck_split [simp]:  "[] \<turnstile>\<^sub>d e : t \<Longrightarrow> [] \<turnstile>\<^sub>g split_vars e : t"
+proof (unfold split_vars_def)
+  assume "[] \<turnstile>\<^sub>d e : t" 
+  hence "concat [] \<turnstile>\<^sub>d e : t" by simp
+  hence "[] \<turnstile>\<^sub>g split_vars' (inv_map_from_env []) e : t" using typecheck_split' by fastforce
+  thus "[] \<turnstile>\<^sub>g split_vars' Map.empty e : t" by simp
+qed
 
 text \<open>The problem arises when we try to map closures (and, for the same reason, the callstack). We 
 have an environment and an expression to be evaluated in that environment; we need to split the 
@@ -120,14 +200,17 @@ next
   ultimately show ?case by simp
 qed simp_all
      
-lemma combine_split_cancel [simp]: "[] \<turnstile>\<^sub>d e : t \<Longrightarrow> combine_vars (split_vars e) = e"
-proof (unfold combine_vars_def split_vars_def)
+lemma combine_split_cancel_empty [simp]: "[] \<turnstile>\<^sub>d e : t \<Longrightarrow> 
+  combine_vars' Map.empty (split_vars' Map.empty e) = e" 
+proof -
   assume "[] \<turnstile>\<^sub>d e : t" 
   moreover have "dom Map.empty = dom (lookup [])" by simp
   moreover have "\<And>x y. Map.empty x = Some y \<Longrightarrow> Map.empty y = Some x" by simp
-  ultimately show "combine_vars' Map.empty (split_vars' Map.empty e) = e" 
-    by (metis combine_split_cancel')
+  ultimately show ?thesis by (metis combine_split_cancel')
 qed
+
+lemma combine_split_cancel [simp]: "[] \<turnstile>\<^sub>d e : t \<Longrightarrow> combine_vars (split_vars e) = e" 
+  by (simp add: combine_vars_def split_vars_def)
 
 lemma split_combine_cancel' [simp]: "\<Gamma> \<turnstile>\<^sub>g e : t \<Longrightarrow> (\<And>x y. \<Phi> x = Some y \<Longrightarrow> \<Phi>' y = Some x) \<Longrightarrow>  
   dom \<Phi> = {xy. \<exists>z. lookup \<Gamma> (fst xy) = Some z \<and> snd xy \<in> dom (lookup z)} \<Longrightarrow>
@@ -164,14 +247,6 @@ next
   case (tc\<^sub>g_let \<Gamma> e\<^sub>1 t\<^sub>1 e\<^sub>2 t\<^sub>2)
   hence X: "\<And>x y. inv_map_past_let \<Phi> x = Some y \<Longrightarrow> map_past_let \<Phi>' y = Some x" 
     using inv_inv_map_past_let_inv by fastforce
-
-  from tc\<^sub>g_let have "\<Gamma> \<turnstile>\<^sub>g e\<^sub>1 : t\<^sub>1" by simp
-  from tc\<^sub>g_let have "cons_fst t\<^sub>1 \<Gamma> \<turnstile>\<^sub>g e\<^sub>2 : t\<^sub>2" by simp
-  from tc\<^sub>g_let have "split_vars' \<Phi>' (combine_vars' \<Phi> e\<^sub>1) = e\<^sub>1" by simp
-  from tc\<^sub>g_let have "\<Phi> xx = Some xy \<Longrightarrow> \<Phi>' xy = Some xx" by simp
-  from tc\<^sub>g_let have "dom \<Phi> = {xy. \<exists>z. lookup \<Gamma> (fst xy) = Some z \<and> snd xy \<in> dom (lookup z)}" by simp
-
-
   have Y: "\<And>xy. xy \<in> insert (0, 0) ((\<lambda>x. case x of (x, y) \<Rightarrow> (x, if x = 0 then Suc y else y)) `
     {xy. \<exists>z. lookup \<Gamma> (fst xy) = Some z \<and> snd xy \<in> dom (lookup z)}) \<Longrightarrow>
     xy \<in> {xy. \<exists>z. (case fst xy of 0 \<Rightarrow> (case lookup \<Gamma> 0 of None \<Rightarrow> Some [t\<^sub>1] 
@@ -220,6 +295,9 @@ fun map_from_env :: "'a list list \<Rightarrow> nat \<times> nat \<rightharpoonu
 | "map_from_env (cs # \<Delta>) (0, y) = (if y < length cs then Some y else None)"
 | "map_from_env (cs # \<Delta>) (Suc x, y) = map_option ((+) (length cs)) (map_from_env \<Delta> (x, y))"
 
+lemma map_from_env_empty [simp]: "map_from_env [] = Map.empty"
+  by auto
+
 lemma lookup_map_from_env [simp]: "lookup \<Delta> x = Some cs \<Longrightarrow> lookup cs y = Some c \<Longrightarrow> 
     map_from_env \<Delta> (x, y) \<noteq> None"
   by (induction \<Delta> "(x, y)" arbitrary: x y rule: map_from_env.induct) simp_all
@@ -242,7 +320,8 @@ primrec combine_frame :: "frame\<^sub>g \<Rightarrow> frame\<^sub>c" where
     FApp1\<^sub>c (concat (map (map combine_closure) \<Delta>)) (combine_vars' (map_from_env \<Delta>) e)"
 | "combine_frame (FApp2\<^sub>g c) = FApp2\<^sub>c (combine_closure c)"
 | "combine_frame (FLet\<^sub>g \<Delta> e) = 
-    FLet\<^sub>c (concat (map (map combine_closure) \<Delta>)) (combine_vars' (map_from_env \<Delta>) e)"
+    FLet\<^sub>c (concat (map (map combine_closure) \<Delta>)) 
+      (combine_vars' (inv_map_past_let (map_from_env \<Delta>)) e)"
 | "combine_frame (FPop\<^sub>g c) = FPop\<^sub>c (combine_closure c)"
 | "combine_frame (FReturn\<^sub>g \<Delta>) = FReturn\<^sub>c (concat (map (map combine_closure) \<Delta>))"
 
@@ -252,8 +331,7 @@ primrec combine_state :: "state\<^sub>g \<Rightarrow> state\<^sub>c" where
       (combine_vars' (map_from_env \<Delta>) e)"
 | "combine_state (SC\<^sub>g s c) = SC\<^sub>c (map combine_frame s) (combine_closure c)"
 
-text \<open>We can now prove our typechecking theorems: note again how the "empty" context cannot really 
-be \<open>[]\<close>, because of the need for a space to put top-level lets in.\<close>
+text \<open>We can now prove our typechecking theorems:\<close>
 
 lemma map_from_env_insert' [simp]: "map_from_env (insert_at 0 [t] \<Gamma>) x = 
     inv_map_past_lam (map_from_env \<Gamma>) x"
@@ -263,11 +341,17 @@ lemma map_from_env_insert [simp]: "map_from_env (insert_at 0 [t] \<Gamma>) =
     inv_map_past_lam (map_from_env \<Gamma>)"
   by auto
 
+lemma map_from_env_insert2 [simp]: "map_from_env ([t] # \<Gamma>) = inv_map_past_lam (map_from_env \<Gamma>)"
+proof -
+  have "map_from_env (insert_at 0 [t] \<Gamma>) = inv_map_past_lam (map_from_env \<Gamma>)" by simp
+  thus ?thesis by (cases \<Gamma>) simp_all
+qed
+
 lemma map_from_env_mapfst' [simp]: "map_from_env (cons_fst t \<Gamma>) x = 
     inv_map_past_let (map_from_env \<Gamma>) x"
 proof (induction \<Gamma> x rule: map_from_env.induct)
   case (1 x y)
-  thus ?case by (cases x) simp_all
+  thus ?case by (cases x) (simp_all split: nat.splits)
 qed (auto simp add: option.map_comp)
 
 lemma map_from_env_mapfst [simp]: "map_from_env (cons_fst t \<Gamma>) = inv_map_past_let (map_from_env \<Gamma>)"
@@ -279,17 +363,17 @@ lemma typecheck_combine [simp]: "\<Gamma> \<turnstile>\<^sub>g e : t \<Longright
 lemma "c :\<^sub>g\<^sub>c\<^sub>l t \<Longrightarrow> True"
   and map_from_env_type_vals' [simp]: "\<Delta> :\<^sub>g\<^sub>c\<^sub>l\<^sub>s \<Gamma> \<Longrightarrow> map_from_env \<Gamma> x = map_from_env \<Delta> x"
 proof (induction c t and \<Delta> \<Gamma> arbitrary: and x rule: typing_closure\<^sub>g_typing_environment\<^sub>g.inducts)
-  case tc\<^sub>c_nil
+  case tc\<^sub>g_nil
   thus ?case by (cases x) simp_all
 next
-  case (tc\<^sub>c_cons_nil \<Delta> \<Gamma>)
+  case (tc\<^sub>g_cons_nil \<Delta> \<Gamma>)
   thus ?case
   proof (induction x)
     case (Pair a b)
     then show ?case by (cases a) simp_all
   qed
 next
-  case (tc\<^sub>c_cons_cons c t cs \<Delta> ts \<Gamma>)
+  case (tc\<^sub>g_cons_cons c t cs \<Delta> ts \<Gamma>)
   thus ?case 
   proof (induction x)
     case (Pair a b)
@@ -312,15 +396,15 @@ lemma typecheck_combine_closure [simp]: "c :\<^sub>g\<^sub>c\<^sub>l t \<Longrig
   and typecheck_concat_combine_closure [simp]: "\<Delta> :\<^sub>g\<^sub>c\<^sub>l\<^sub>s \<Gamma> \<Longrightarrow> 
     concat (map (map combine_closure) \<Delta>) :\<^sub>c\<^sub>l\<^sub>s concat \<Gamma>"
 proof (induction c t and \<Delta> \<Gamma> rule: typing_closure\<^sub>g_typing_environment\<^sub>g.inducts)
-  case (tc\<^sub>c_lam \<Delta> \<Gamma> t\<^sub>1 e t\<^sub>2)
+  case (tc\<^sub>g_lam \<Delta> \<Gamma> t\<^sub>1 e t\<^sub>2)
   hence X: "map_from_env \<Gamma> = map_from_env \<Delta>" by simp
-  from tc\<^sub>c_lam have "concat (insert_at 0 [t\<^sub>1] \<Gamma>) \<turnstile>\<^sub>d 
+  from tc\<^sub>g_lam have "concat (insert_at 0 [t\<^sub>1] \<Gamma>) \<turnstile>\<^sub>d 
     combine_vars' (map_from_env (insert_at 0 [t\<^sub>1] \<Gamma>)) e : t\<^sub>2" by (metis typecheck_combine)
   hence "insert_at 0 t\<^sub>1 (concat \<Gamma>) \<turnstile>\<^sub>d combine_vars' (inv_map_past_lam (map_from_env \<Gamma>)) e : t\<^sub>2" 
     by simp
   hence "insert_at 0 t\<^sub>1 (concat \<Gamma>) \<turnstile>\<^sub>d combine_vars' (inv_map_past_lam (map_from_env \<Delta>)) e : t\<^sub>2" 
     using X by metis
-  with tc\<^sub>c_lam show ?case by simp
+  with tc\<^sub>g_lam show ?case by simp
 qed simp_all
 
 lemma combine_clsoure_mapfst [simp]: "concat (map (map combine_closure) (cons_fst c \<Delta>)) = 
@@ -336,28 +420,282 @@ qed simp_all
 
 lemma typecheck_stack [simp]: "s :\<^sub>g t\<^sub>2 \<rightarrow> t \<Longrightarrow> map combine_frame s :\<^sub>c t\<^sub>2 \<rightarrow> t"
 proof (induction s t\<^sub>2 t rule: typing_stack\<^sub>g.induct)
-  case (tcc_scons_app1 \<Delta> \<Gamma> e t\<^sub>1 s t\<^sub>2 t)
+  case (tcg_scons_app1 \<Delta> \<Gamma> e t\<^sub>1 s t\<^sub>2 t)
   hence X: "concat (map (map combine_closure) \<Delta>) :\<^sub>c\<^sub>l\<^sub>s concat \<Gamma>" by simp
-  from tcc_scons_app1 have "map_from_env \<Delta> = map_from_env \<Gamma>" by simp
-  with tcc_scons_app1(2) have Y: "concat \<Gamma> \<turnstile>\<^sub>d combine_vars' (map_from_env \<Delta>) e : t\<^sub>1" by simp
-  from tcc_scons_app1 have "latest_environment\<^sub>c (map combine_frame s) = 
+  from tcg_scons_app1 have "map_from_env \<Delta> = map_from_env \<Gamma>" by simp
+  with tcg_scons_app1(2) have Y: "concat \<Gamma> \<turnstile>\<^sub>d combine_vars' (map_from_env \<Delta>) e : t\<^sub>1" by simp
+  from tcg_scons_app1 have "latest_environment\<^sub>c (map combine_frame s) = 
     Some (concat (map (map combine_closure) \<Delta>))" by simp
-  with tcc_scons_app1 X Y have "FApp1\<^sub>c (concat (map (map combine_closure) \<Delta>)) 
-    (combine_vars' (map_from_env \<Delta>) e) # map combine_frame s :\<^sub>c Arrow t\<^sub>1 t\<^sub>2 \<rightarrow> t" 
-      by (metis typing_stack\<^sub>c.tcc_scons_app1)
-  thus ?case by simp
+  with tcg_scons_app1(5) X Y show ?case by simp
 next
-  case (tcc_scons_app2 c t\<^sub>1 t\<^sub>2 s t)
-  then show ?case by simp
+  case (tcg_scons_app2 c t\<^sub>1 t\<^sub>2 s t)
+  hence "combine_closure c :\<^sub>c\<^sub>l Arrow t\<^sub>1 t\<^sub>2" by simp
+  moreover from tcg_scons_app2 have "map combine_frame s :\<^sub>c t\<^sub>2 \<rightarrow> t" by simp
+  moreover from tcg_scons_app2 have "latest_environment\<^sub>c (map combine_frame s) \<noteq> None" by simp
+  ultimately show ?case by simp
 next
-  case (tcc_scons_let s \<Delta> \<Gamma> t\<^sub>1 e t\<^sub>2 t)
-  then show ?case by simp
+  case (tcg_scons_let s \<Delta> \<Gamma> t\<^sub>1 e t\<^sub>2 t)
+  hence "concat (cons_fst t\<^sub>1 \<Gamma>) \<turnstile>\<^sub>d combine_vars' (map_from_env (cons_fst t\<^sub>1 \<Gamma>)) e : t\<^sub>2" 
+    by (metis typecheck_combine)
+  hence X: "insert_at 0 t\<^sub>1 (concat \<Gamma>) \<turnstile>\<^sub>d combine_vars' (inv_map_past_let (map_from_env \<Gamma>)) e : t\<^sub>2"
+    by simp
+  from tcg_scons_let have "map_from_env \<Delta> = map_from_env \<Gamma>" by simp
+  with X have "insert_at 0 t\<^sub>1 (concat \<Gamma>) \<turnstile>\<^sub>d 
+    combine_vars' (inv_map_past_let (map_from_env \<Delta>)) e : t\<^sub>2" by metis
+  moreover from tcg_scons_let have "latest_environment\<^sub>c (map combine_frame s) = 
+    Some (concat (map (map combine_closure) \<Delta>))" by simp
+  moreover from tcg_scons_let have "concat (map (map combine_closure) \<Delta>) :\<^sub>c\<^sub>l\<^sub>s concat \<Gamma>" by simp
+  moreover from tcg_scons_let have "map combine_frame s :\<^sub>c t\<^sub>2 \<rightarrow> t" by simp
+  ultimately show ?case by simp
 next
-  case (tcc_scons_pop s \<Delta> c tt t' t)
-  then show ?case by simp
+  case (tcg_scons_pop s c tt t' t)
+  hence "latest_environment\<^sub>c (map combine_frame s) \<noteq> None" by simp
+  moreover from tcg_scons_pop have "combine_closure c :\<^sub>c\<^sub>l tt" by simp
+  moreover from tcg_scons_pop have "map combine_frame s :\<^sub>c t' \<rightarrow> t" by simp
+  ultimately show ?case by simp
 next
-  case (tcc_scons_ret \<Delta> \<Gamma> s t' t)
-  then show ?case by simp
+  case (tcg_scons_ret \<Delta> \<Gamma> s t' t)
+  hence "concat (map (map combine_closure) \<Delta>) :\<^sub>c\<^sub>l\<^sub>s concat \<Gamma>" by simp
+  moreover from tcg_scons_ret have "map combine_frame s :\<^sub>c t' \<rightarrow> t" by simp
+  ultimately show ?case by simp
 qed simp_all
-                                  
+
+lemma typecheck_state [simp]: "\<Sigma> :\<^sub>g t \<Longrightarrow> combine_state \<Sigma> :\<^sub>c t"
+proof (induction \<Sigma> t rule: typecheck_state\<^sub>g.induct)
+  case (tcg_state_ev s t' t \<Delta> \<Gamma> e)
+  hence "concat \<Gamma> \<turnstile>\<^sub>d combine_vars' (map_from_env \<Gamma>) e : t'" 
+    by (metis typecheck_combine)
+  with tcg_state_ev have "concat \<Gamma> \<turnstile>\<^sub>d combine_vars' (map_from_env \<Delta>) e : t'" by simp
+  moreover from tcg_state_ev have "map combine_frame s :\<^sub>c t' \<rightarrow> t" by simp
+  moreover from tcg_state_ev have "concat (map (map combine_closure) \<Delta>) :\<^sub>c\<^sub>l\<^sub>s concat \<Gamma>" by simp
+  moreover from tcg_state_ev have "latest_environment\<^sub>c (map combine_frame s) = 
+    Some (concat (map (map combine_closure) \<Delta>))" by simp
+  ultimately show ?case by simp
+next
+  case (tcg_state_ret s t' t c)
+  hence "map combine_frame s :\<^sub>c t' \<rightarrow> t" by simp
+  moreover from tcg_state_ret have "combine_closure c :\<^sub>c\<^sub>l t'" by simp
+  ultimately show ?case by simp
+qed
+
+text \<open>Now, the evaluation correctness theorems. As usual, one way is much simpler than the other.\<close>
+
+theorem completeness\<^sub>g [simp]: "\<Sigma> \<leadsto>\<^sub>g \<Sigma>' \<Longrightarrow> combine_state \<Sigma> \<leadsto>\<^sub>c combine_state \<Sigma>'"
+proof (induction \<Sigma> \<Sigma>' rule: eval\<^sub>g.induct)
+  case (ev\<^sub>g_var \<Delta> x cs y c s)
+  hence "lookup (map combine_closure (concat \<Delta>)) (the (map_from_env \<Delta> (x, y))) = 
+    Some (combine_closure c)" by simp
+  thus ?case by (simp add: map_concat) 
+qed simp_all
+
+lemma combine_to_var [dest]: "\<Gamma> \<turnstile>\<^sub>g e\<^sub>g : t \<Longrightarrow> Var\<^sub>d x = combine_vars' (map_from_env \<Delta>) e\<^sub>g \<Longrightarrow> 
+    \<Delta> :\<^sub>g\<^sub>c\<^sub>l\<^sub>s \<Gamma> \<Longrightarrow> \<exists>y z. e\<^sub>g = Var\<^sub>g y z \<and> map_from_env \<Delta> (y, z) = Some x"
+proof (induction \<Gamma> e\<^sub>g t rule: typing\<^sub>g.induct) 
+  case (tc\<^sub>g_var \<Gamma> x ts y t)
+  hence "map_from_env \<Delta> = map_from_env \<Gamma>" by simp
+  with tc\<^sub>g_var have "map_from_env \<Delta> (x, y) \<noteq> None" by (metis lookup_map_from_env)
+  with tc\<^sub>g_var show ?case by simp
+qed simp_all
+ 
+lemma combine_to_con [dest]: "Const\<^sub>d n = combine_vars' \<Phi> e\<^sub>g \<Longrightarrow> e\<^sub>g = Const\<^sub>g n"
+  by (induction e\<^sub>g) simp_all
+
+lemma combine_to_lam [dest]: "Lam\<^sub>d t e\<^sub>c = combine_vars' \<Phi> e\<^sub>g \<Longrightarrow> 
+    \<exists>e\<^sub>g' n. e\<^sub>g = Lam\<^sub>g t e\<^sub>g' n \<and> e\<^sub>c = combine_vars' (inv_map_past_lam \<Phi>) e\<^sub>g'"
+  by (induction e\<^sub>g) simp_all
+
+lemma combine_to_app [dest]: "App\<^sub>d e\<^sub>1\<^sub>c e\<^sub>2\<^sub>c = combine_vars' \<Phi> e\<^sub>g \<Longrightarrow> 
+    \<exists>e\<^sub>1\<^sub>g e\<^sub>2\<^sub>g. e\<^sub>g = App\<^sub>g e\<^sub>1\<^sub>g e\<^sub>2\<^sub>g \<and> e\<^sub>1\<^sub>c = combine_vars' \<Phi> e\<^sub>1\<^sub>g \<and> e\<^sub>2\<^sub>c = combine_vars' \<Phi> e\<^sub>2\<^sub>g"
+  by (induction e\<^sub>g) simp_all
+
+lemma combine_to_let [dest]: "Let\<^sub>d e\<^sub>1\<^sub>c e\<^sub>2\<^sub>c = combine_vars' \<Phi> e\<^sub>g \<Longrightarrow> 
+  \<exists>e\<^sub>1\<^sub>g e\<^sub>2\<^sub>g. e\<^sub>g = Let\<^sub>g e\<^sub>1\<^sub>g e\<^sub>2\<^sub>g \<and> e\<^sub>1\<^sub>c = combine_vars' \<Phi> e\<^sub>1\<^sub>g \<and> 
+    e\<^sub>2\<^sub>c = combine_vars' (inv_map_past_let \<Phi>) e\<^sub>2\<^sub>g"
+  by (induction e\<^sub>g) simp_all
+
+lemma combine_to_lamc [dest]: "Lam\<^sub>c t \<Delta>\<^sub>c e\<^sub>c = combine_closure c\<^sub>g \<Longrightarrow> 
+  \<exists>\<Delta>\<^sub>g e\<^sub>g n. c\<^sub>g = Fun\<^sub>g t \<Delta>\<^sub>g e\<^sub>g n \<and> \<Delta>\<^sub>c = concat (map (map combine_closure) \<Delta>\<^sub>g) \<and> 
+    e\<^sub>c = combine_vars' (inv_map_past_lam (map_from_env \<Delta>\<^sub>g)) e\<^sub>g"
+  by (induction c\<^sub>g) simp_all
+
+lemma combine_to_fapp1 [dest]: "FApp1\<^sub>c \<Delta>\<^sub>c e\<^sub>c = combine_frame f\<^sub>g \<Longrightarrow> 
+  \<exists>\<Delta>\<^sub>g e\<^sub>g. f\<^sub>g = FApp1\<^sub>g \<Delta>\<^sub>g e\<^sub>g \<and> \<Delta>\<^sub>c = concat (map (map combine_closure) \<Delta>\<^sub>g) \<and> 
+    e\<^sub>c = combine_vars' (map_from_env \<Delta>\<^sub>g) e\<^sub>g"
+  by (induction f\<^sub>g) simp_all
+
+lemma combine_to_fapp2 [dest]: "FApp2\<^sub>c c\<^sub>c = combine_frame f\<^sub>g \<Longrightarrow> 
+  \<exists>c\<^sub>g. f\<^sub>g = FApp2\<^sub>g c\<^sub>g \<and> c\<^sub>c = combine_closure c\<^sub>g"
+  by (induction f\<^sub>g) simp_all
+
+lemma combine_to_flet [dest]: "FLet\<^sub>c \<Delta>\<^sub>c e\<^sub>c = combine_frame f\<^sub>g \<Longrightarrow> 
+  \<exists>\<Delta>\<^sub>g e\<^sub>g. f\<^sub>g = FLet\<^sub>g \<Delta>\<^sub>g e\<^sub>g \<and> \<Delta>\<^sub>c = concat (map (map combine_closure) \<Delta>\<^sub>g) \<and> 
+    e\<^sub>c = combine_vars' (inv_map_past_let (map_from_env \<Delta>\<^sub>g)) e\<^sub>g"
+  by (induction f\<^sub>g) simp_all
+
+lemma combine_to_fpop [dest]: "FPop\<^sub>c c\<^sub>c = combine_frame f\<^sub>g \<Longrightarrow> 
+  \<exists>c\<^sub>g. f\<^sub>g = FPop\<^sub>g c\<^sub>g \<and> c\<^sub>c = combine_closure c\<^sub>g"
+  by (induction f\<^sub>g) simp_all
+
+lemma combine_to_freturn [dest]: "FReturn\<^sub>c \<Delta>\<^sub>c = combine_frame f\<^sub>g \<Longrightarrow> 
+    \<exists>\<Delta>\<^sub>g. f\<^sub>g = FReturn\<^sub>g \<Delta>\<^sub>g \<and> \<Delta>\<^sub>c = concat (map (map combine_closure) \<Delta>\<^sub>g)"
+  by (induction f\<^sub>g) simp_all
+
+lemma combine_to_eval_state [dest]: "SE\<^sub>c s\<^sub>c \<Delta>\<^sub>c e\<^sub>c = combine_state \<Sigma>\<^sub>g \<Longrightarrow> 
+  \<exists>s\<^sub>g \<Delta>\<^sub>g e\<^sub>g. \<Sigma>\<^sub>g = SE\<^sub>g s\<^sub>g \<Delta>\<^sub>g e\<^sub>g \<and> s\<^sub>c = map combine_frame s\<^sub>g \<and> 
+    \<Delta>\<^sub>c = concat (map (map combine_closure) \<Delta>\<^sub>g) \<and> e\<^sub>c = combine_vars' (map_from_env \<Delta>\<^sub>g) e\<^sub>g"
+  by (induction \<Sigma>\<^sub>g) simp_all
+
+lemma combine_to_return_state [dest]: "SC\<^sub>c s\<^sub>c c\<^sub>c = combine_state \<Sigma>\<^sub>g \<Longrightarrow> 
+    \<exists>s\<^sub>g c\<^sub>g. \<Sigma>\<^sub>g = SC\<^sub>g s\<^sub>g c\<^sub>g \<and> s\<^sub>c = map combine_frame s\<^sub>g \<and> c\<^sub>c = combine_closure c\<^sub>g"
+  by (induction \<Sigma>\<^sub>g) simp_all
+
+lemma lookup_map_inv [simp]: "map_from_env \<Delta> (y, z) = Some x \<Longrightarrow>
+  lookup (concat (map (map combine_closure) \<Delta>)) x = Some c \<Longrightarrow> 
+    \<exists>cs c\<^sub>g. lookup \<Delta> y = Some cs \<and> lookup cs z = Some c\<^sub>g \<and> c = combine_closure c\<^sub>g" 
+  by (induction \<Delta> "(y, z)" arbitrary: x y z rule: map_from_env.induct) (auto split: if_splits)
+
+theorem correctness\<^sub>g [simp]: "combine_state \<Sigma>\<^sub>g \<leadsto>\<^sub>c \<Sigma>\<^sub>c' \<Longrightarrow> \<Sigma>\<^sub>g :\<^sub>g t \<Longrightarrow>
+  \<exists>\<Sigma>\<^sub>g'. \<Sigma>\<^sub>g \<leadsto>\<^sub>g \<Sigma>\<^sub>g' \<and> \<Sigma>\<^sub>c' = combine_state \<Sigma>\<^sub>g'"
+proof (induction "combine_state \<Sigma>\<^sub>g" \<Sigma>\<^sub>c' rule: eval\<^sub>c.induct)
+  case (ev\<^sub>c_var \<Delta>\<^sub>c x c\<^sub>c s\<^sub>c)
+  then obtain s\<^sub>g \<Delta>\<^sub>g e\<^sub>g where S: "\<Sigma>\<^sub>g = SE\<^sub>g s\<^sub>g \<Delta>\<^sub>g e\<^sub>g \<and> s\<^sub>c = map combine_frame s\<^sub>g \<and> 
+    \<Delta>\<^sub>c = concat (map (map combine_closure) \<Delta>\<^sub>g) \<and> Var\<^sub>d x = combine_vars' (map_from_env \<Delta>\<^sub>g) e\<^sub>g" 
+      by auto
+  with ev\<^sub>c_var obtain t' \<Gamma> where "(s\<^sub>g :\<^sub>g t' \<rightarrow> t) \<and> (\<Delta>\<^sub>g :\<^sub>g\<^sub>c\<^sub>l\<^sub>s \<Gamma>) \<and> 
+    latest_environment\<^sub>g s\<^sub>g = Some \<Delta>\<^sub>g \<and> \<Gamma> \<turnstile>\<^sub>g e\<^sub>g : t'" by auto
+  with S obtain y z where Y: "e\<^sub>g = Var\<^sub>g y z \<and> map_from_env \<Delta>\<^sub>g (y, z) = Some x" by auto
+  from ev\<^sub>c_var S have "lookup (concat (map (map combine_closure) \<Delta>\<^sub>g)) x = Some c\<^sub>c" by blast
+  with Y obtain cs c\<^sub>g where "lookup \<Delta>\<^sub>g y = Some cs \<and> lookup cs z = Some c\<^sub>g \<and> c\<^sub>c = combine_closure c\<^sub>g" 
+    using lookup_map_inv by blast
+  with S have "SE\<^sub>g s\<^sub>g \<Delta>\<^sub>g (Var\<^sub>g y z) \<leadsto>\<^sub>g SC\<^sub>g s\<^sub>g c\<^sub>g \<and> SC\<^sub>c s\<^sub>c c\<^sub>c = combine_state (SC\<^sub>g s\<^sub>g c\<^sub>g)" by simp
+  with S Y show ?case by blast
+next
+  case (ev\<^sub>c_con s\<^sub>c \<Delta>\<^sub>c n)
+  then obtain s\<^sub>g \<Delta>\<^sub>g where "\<Sigma>\<^sub>g = SE\<^sub>g s\<^sub>g \<Delta>\<^sub>g (Const\<^sub>g n) \<and> s\<^sub>c = map combine_frame s\<^sub>g \<and> 
+    \<Delta>\<^sub>c = concat (map (map combine_closure) \<Delta>\<^sub>g)" by blast
+  moreover hence "SE\<^sub>g s\<^sub>g \<Delta>\<^sub>g (Const\<^sub>g n) \<leadsto>\<^sub>g SC\<^sub>g s\<^sub>g (Num\<^sub>g n) \<and> 
+    SC\<^sub>c s\<^sub>c (Const\<^sub>c n) = combine_state (SC\<^sub>g s\<^sub>g (Num\<^sub>g n))" by simp
+  ultimately show ?case by blast
+next
+  case (ev\<^sub>c_lam s\<^sub>c \<Delta>\<^sub>c t e\<^sub>c)
+  then obtain s\<^sub>g \<Delta>\<^sub>g e\<^sub>g where S: "\<Sigma>\<^sub>g = SE\<^sub>g s\<^sub>g \<Delta>\<^sub>g e\<^sub>g \<and> s\<^sub>c = map combine_frame s\<^sub>g \<and> 
+    \<Delta>\<^sub>c = concat (map (map combine_closure) \<Delta>\<^sub>g) \<and> Lam\<^sub>d t e\<^sub>c = combine_vars' (map_from_env \<Delta>\<^sub>g) e\<^sub>g" 
+      by auto
+  moreover then obtain e\<^sub>g' n where "e\<^sub>g = Lam\<^sub>g t e\<^sub>g' n \<and> 
+    e\<^sub>c = combine_vars' (inv_map_past_lam (map_from_env \<Delta>\<^sub>g)) e\<^sub>g'" by auto
+  moreover with S have "SE\<^sub>g s\<^sub>g \<Delta>\<^sub>g (Lam\<^sub>g t e\<^sub>g' n) \<leadsto>\<^sub>g SC\<^sub>g s\<^sub>g (Fun\<^sub>g t \<Delta>\<^sub>g e\<^sub>g' n) \<and> 
+    SC\<^sub>c s\<^sub>c (Lam\<^sub>c t \<Delta>\<^sub>c e\<^sub>c) = combine_state (SC\<^sub>g s\<^sub>g (Fun\<^sub>g t \<Delta>\<^sub>g e\<^sub>g' n))" by simp
+  ultimately show ?case by blast
+next
+  case (ev\<^sub>c_app s\<^sub>c \<Delta>\<^sub>c e\<^sub>1\<^sub>c e\<^sub>2\<^sub>c)
+  then obtain s\<^sub>g \<Delta>\<^sub>g e\<^sub>g where S: "\<Sigma>\<^sub>g = SE\<^sub>g s\<^sub>g \<Delta>\<^sub>g e\<^sub>g \<and> s\<^sub>c = map combine_frame s\<^sub>g \<and> 
+    \<Delta>\<^sub>c = concat (map (map combine_closure) \<Delta>\<^sub>g) \<and> App\<^sub>d e\<^sub>1\<^sub>c e\<^sub>2\<^sub>c = combine_vars' (map_from_env \<Delta>\<^sub>g) e\<^sub>g" 
+      by auto
+  moreover then obtain e\<^sub>1\<^sub>g e\<^sub>2\<^sub>g where "e\<^sub>g = App\<^sub>g e\<^sub>1\<^sub>g e\<^sub>2\<^sub>g \<and> e\<^sub>1\<^sub>c = combine_vars' (map_from_env \<Delta>\<^sub>g) e\<^sub>1\<^sub>g \<and> 
+    e\<^sub>2\<^sub>c = combine_vars' (map_from_env \<Delta>\<^sub>g) e\<^sub>2\<^sub>g" by auto
+  moreover with S have "SE\<^sub>g s\<^sub>g \<Delta>\<^sub>g (App\<^sub>g e\<^sub>1\<^sub>g e\<^sub>2\<^sub>g) \<leadsto>\<^sub>g SE\<^sub>g (FApp1\<^sub>g \<Delta>\<^sub>g e\<^sub>2\<^sub>g # s\<^sub>g) \<Delta>\<^sub>g e\<^sub>1\<^sub>g \<and> 
+    SE\<^sub>c (FApp1\<^sub>c \<Delta>\<^sub>c e\<^sub>2\<^sub>c # s\<^sub>c) \<Delta>\<^sub>c e\<^sub>1\<^sub>c = combine_state (SE\<^sub>g (FApp1\<^sub>g \<Delta>\<^sub>g e\<^sub>2\<^sub>g # s\<^sub>g) \<Delta>\<^sub>g e\<^sub>1\<^sub>g)" by simp
+  ultimately show ?case by blast
+next
+  case (ev\<^sub>c_let s\<^sub>c \<Delta>\<^sub>c e\<^sub>1\<^sub>c e\<^sub>2\<^sub>c)
+  then obtain s\<^sub>g \<Delta>\<^sub>g e\<^sub>g where S: "\<Sigma>\<^sub>g = SE\<^sub>g s\<^sub>g \<Delta>\<^sub>g e\<^sub>g \<and> s\<^sub>c = map combine_frame s\<^sub>g \<and> 
+    \<Delta>\<^sub>c = concat (map (map combine_closure) \<Delta>\<^sub>g) \<and> Let\<^sub>d e\<^sub>1\<^sub>c e\<^sub>2\<^sub>c = combine_vars' (map_from_env \<Delta>\<^sub>g) e\<^sub>g" 
+      by auto
+  moreover then obtain e\<^sub>1\<^sub>g e\<^sub>2\<^sub>g where "e\<^sub>g = Let\<^sub>g e\<^sub>1\<^sub>g e\<^sub>2\<^sub>g \<and> e\<^sub>1\<^sub>c = combine_vars' (map_from_env \<Delta>\<^sub>g) e\<^sub>1\<^sub>g \<and> 
+    e\<^sub>2\<^sub>c = combine_vars' (inv_map_past_let (map_from_env \<Delta>\<^sub>g)) e\<^sub>2\<^sub>g" by auto
+  moreover with S have "SE\<^sub>g s\<^sub>g \<Delta>\<^sub>g (Let\<^sub>g e\<^sub>1\<^sub>g e\<^sub>2\<^sub>g) \<leadsto>\<^sub>g SE\<^sub>g (FLet\<^sub>g \<Delta>\<^sub>g e\<^sub>2\<^sub>g # s\<^sub>g) \<Delta>\<^sub>g e\<^sub>1\<^sub>g \<and> 
+    SE\<^sub>c (FLet\<^sub>c \<Delta>\<^sub>c e\<^sub>2\<^sub>c # s\<^sub>c) \<Delta>\<^sub>c e\<^sub>1\<^sub>c = combine_state (SE\<^sub>g (FLet\<^sub>g \<Delta>\<^sub>g e\<^sub>2\<^sub>g # s\<^sub>g) \<Delta>\<^sub>g e\<^sub>1\<^sub>g)" by simp
+  ultimately show ?case by blast
+next
+  case (ret\<^sub>c_app1 \<Delta>\<^sub>c e\<^sub>c s\<^sub>c c\<^sub>c)
+  then obtain s\<^sub>g' c\<^sub>g where S: "\<Sigma>\<^sub>g = SC\<^sub>g s\<^sub>g' c\<^sub>g \<and> FApp1\<^sub>c \<Delta>\<^sub>c e\<^sub>c # s\<^sub>c = map combine_frame s\<^sub>g' \<and> 
+    c\<^sub>c = combine_closure c\<^sub>g" by blast
+  moreover then obtain f\<^sub>g s\<^sub>g where F: "FApp1\<^sub>c \<Delta>\<^sub>c e\<^sub>c = combine_frame f\<^sub>g \<and> s\<^sub>c = map combine_frame s\<^sub>g \<and> 
+    s\<^sub>g' = f\<^sub>g # s\<^sub>g" by blast
+  moreover then obtain \<Delta>\<^sub>g e\<^sub>g where "f\<^sub>g = FApp1\<^sub>g \<Delta>\<^sub>g e\<^sub>g \<and> \<Delta>\<^sub>c = concat (map (map combine_closure) \<Delta>\<^sub>g) \<and> 
+    e\<^sub>c = combine_vars' (map_from_env \<Delta>\<^sub>g) e\<^sub>g" by blast
+  moreover with S F have "SC\<^sub>g (FApp1\<^sub>g \<Delta>\<^sub>g e\<^sub>g # s\<^sub>g) c\<^sub>g \<leadsto>\<^sub>g SE\<^sub>g (FApp2\<^sub>g c\<^sub>g # s\<^sub>g) \<Delta>\<^sub>g e\<^sub>g \<and> 
+    SE\<^sub>c (FApp2\<^sub>c c\<^sub>c # s\<^sub>c) \<Delta>\<^sub>c e\<^sub>c = combine_state (SE\<^sub>g (FApp2\<^sub>g c\<^sub>g # s\<^sub>g) \<Delta>\<^sub>g e\<^sub>g)" by simp
+  ultimately show ?case by blast
+next
+  case (ret\<^sub>c_app2 t \<Delta>\<^sub>c e\<^sub>c s\<^sub>c c\<^sub>c)
+  then obtain s\<^sub>g' c\<^sub>g where S: "\<Sigma>\<^sub>g = SC\<^sub>g s\<^sub>g' c\<^sub>g \<and> FApp2\<^sub>c (Lam\<^sub>c t \<Delta>\<^sub>c e\<^sub>c) # s\<^sub>c = map combine_frame s\<^sub>g' \<and> 
+    c\<^sub>c = combine_closure c\<^sub>g" by blast
+  moreover then obtain f\<^sub>g s\<^sub>g where F: "FApp2\<^sub>c (Lam\<^sub>c t \<Delta>\<^sub>c e\<^sub>c) = combine_frame f\<^sub>g \<and> 
+    s\<^sub>c = map combine_frame s\<^sub>g \<and> s\<^sub>g' = f\<^sub>g # s\<^sub>g" by blast
+  moreover then obtain c\<^sub>g' where E: "f\<^sub>g = FApp2\<^sub>g c\<^sub>g' \<and> Lam\<^sub>c t \<Delta>\<^sub>c e\<^sub>c = combine_closure c\<^sub>g'" by blast
+  moreover then obtain \<Delta>\<^sub>g e\<^sub>g n where "c\<^sub>g' = Fun\<^sub>g t \<Delta>\<^sub>g e\<^sub>g n \<and> 
+    \<Delta>\<^sub>c = concat (map (map combine_closure) \<Delta>\<^sub>g) \<and> 
+      e\<^sub>c = combine_vars' (inv_map_past_lam (map_from_env \<Delta>\<^sub>g)) e\<^sub>g" by blast
+  moreover with S F E have "SC\<^sub>g (FApp2\<^sub>g (Fun\<^sub>g t \<Delta>\<^sub>g e\<^sub>g n) # s\<^sub>g) c\<^sub>g \<leadsto>\<^sub>g 
+    SE\<^sub>g (FReturn\<^sub>g ([c\<^sub>g] # \<Delta>\<^sub>g) # s\<^sub>g) ([c\<^sub>g] # \<Delta>\<^sub>g) e\<^sub>g \<and> 
+    SE\<^sub>c (FReturn\<^sub>c (c\<^sub>c # \<Delta>\<^sub>c) # s\<^sub>c) (c\<^sub>c # \<Delta>\<^sub>c) e\<^sub>c = 
+      combine_state (SE\<^sub>g (FReturn\<^sub>g ([c\<^sub>g] # \<Delta>\<^sub>g) # s\<^sub>g) ([c\<^sub>g] # \<Delta>\<^sub>g) e\<^sub>g)" by simp
+  ultimately show ?case by blast
+next
+  case (ret\<^sub>c_let \<Delta>\<^sub>c e\<^sub>c s\<^sub>c c\<^sub>c)
+  then obtain s\<^sub>g' c\<^sub>g where S: "\<Sigma>\<^sub>g = SC\<^sub>g s\<^sub>g' c\<^sub>g \<and> FLet\<^sub>c \<Delta>\<^sub>c e\<^sub>c # s\<^sub>c = map combine_frame s\<^sub>g' \<and> 
+    c\<^sub>c = combine_closure c\<^sub>g" by blast
+  moreover then obtain f\<^sub>g s\<^sub>g where F: "FLet\<^sub>c \<Delta>\<^sub>c e\<^sub>c = combine_frame f\<^sub>g \<and> 
+    s\<^sub>c = map combine_frame s\<^sub>g \<and> s\<^sub>g' = f\<^sub>g # s\<^sub>g" by blast
+  moreover then obtain \<Delta>\<^sub>g e\<^sub>g where "f\<^sub>g = FLet\<^sub>g \<Delta>\<^sub>g e\<^sub>g \<and> \<Delta>\<^sub>c = concat (map (map combine_closure) \<Delta>\<^sub>g) \<and> 
+    e\<^sub>c = combine_vars' (inv_map_past_let (map_from_env \<Delta>\<^sub>g)) e\<^sub>g" by blast
+  moreover with S F have "SC\<^sub>g (FLet\<^sub>g \<Delta>\<^sub>g e\<^sub>g # s\<^sub>g) c\<^sub>g \<leadsto>\<^sub>g SE\<^sub>g (FPop\<^sub>g c\<^sub>g # s\<^sub>g) (cons_fst c\<^sub>g \<Delta>\<^sub>g) e\<^sub>g \<and> 
+    SE\<^sub>c (FPop\<^sub>c c\<^sub>c # s\<^sub>c) (c\<^sub>c # \<Delta>\<^sub>c) e\<^sub>c = combine_state (SE\<^sub>g (FPop\<^sub>g c\<^sub>g # s\<^sub>g) (cons_fst c\<^sub>g \<Delta>\<^sub>g) e\<^sub>g)" 
+      by simp
+  ultimately show ?case by blast
+next
+  case (ret\<^sub>c_pop c\<^sub>c' s\<^sub>c c\<^sub>c)
+  then obtain s\<^sub>g' c\<^sub>g where S: "\<Sigma>\<^sub>g = SC\<^sub>g s\<^sub>g' c\<^sub>g \<and> FPop\<^sub>c c\<^sub>c' # s\<^sub>c = map combine_frame s\<^sub>g' \<and> 
+    c\<^sub>c = combine_closure c\<^sub>g" by blast
+  moreover then obtain f\<^sub>g s\<^sub>g where F: "FPop\<^sub>c c\<^sub>c' = combine_frame f\<^sub>g \<and> 
+    s\<^sub>c = map combine_frame s\<^sub>g \<and> s\<^sub>g' = f\<^sub>g # s\<^sub>g" by blast
+  moreover then obtain c\<^sub>g' where "f\<^sub>g = FPop\<^sub>g c\<^sub>g' \<and> c\<^sub>c' = combine_closure c\<^sub>g'" by blast
+  moreover with S F have "SC\<^sub>g (FPop\<^sub>g c\<^sub>g' # s\<^sub>g) c\<^sub>g \<leadsto>\<^sub>g SC\<^sub>g s\<^sub>g c\<^sub>g \<and> 
+    SC\<^sub>c s\<^sub>c c\<^sub>c = combine_state (SC\<^sub>g s\<^sub>g c\<^sub>g)" by simp
+  ultimately show ?case by blast
+next
+  case (ret\<^sub>c_ret \<Delta>\<^sub>c s\<^sub>c c\<^sub>c)
+  then obtain s\<^sub>g' c\<^sub>g where S: "\<Sigma>\<^sub>g = SC\<^sub>g s\<^sub>g' c\<^sub>g \<and> FReturn\<^sub>c \<Delta>\<^sub>c # s\<^sub>c = map combine_frame s\<^sub>g' \<and> 
+    c\<^sub>c = combine_closure c\<^sub>g" by blast
+  moreover then obtain f\<^sub>g s\<^sub>g where F: "FReturn\<^sub>c \<Delta>\<^sub>c = combine_frame f\<^sub>g \<and> 
+    s\<^sub>c = map combine_frame s\<^sub>g \<and> s\<^sub>g' = f\<^sub>g # s\<^sub>g" by blast
+  moreover then obtain \<Delta>\<^sub>g where "f\<^sub>g = FReturn\<^sub>g \<Delta>\<^sub>g \<and> \<Delta>\<^sub>c = concat (map (map combine_closure) \<Delta>\<^sub>g)" 
+    by blast
+  moreover with S F have "SC\<^sub>g (FReturn\<^sub>g \<Delta>\<^sub>g # s\<^sub>g) c\<^sub>g \<leadsto>\<^sub>g SC\<^sub>g s\<^sub>g c\<^sub>g \<and> 
+    SC\<^sub>c s\<^sub>c c\<^sub>c = combine_state (SC\<^sub>g s\<^sub>g c\<^sub>g)" by simp
+  ultimately show ?case by blast
+qed
+
+lemma iter_correctness\<^sub>g [simp]: "iter (\<leadsto>\<^sub>c) (combine_state \<Sigma>\<^sub>g) \<Sigma>\<^sub>c' \<Longrightarrow> \<Sigma>\<^sub>g :\<^sub>g t \<Longrightarrow>
+  \<exists>\<Sigma>\<^sub>g'. iter (\<leadsto>\<^sub>g) \<Sigma>\<^sub>g \<Sigma>\<^sub>g' \<and> \<Sigma>\<^sub>c' = combine_state \<Sigma>\<^sub>g'"
+proof (induction "combine_state \<Sigma>\<^sub>g" \<Sigma>\<^sub>c' arbitrary: \<Sigma>\<^sub>g rule: iter.induct)
+  case iter_refl
+  have "iter (\<leadsto>\<^sub>g) \<Sigma>\<^sub>g \<Sigma>\<^sub>g \<and> combine_state \<Sigma>\<^sub>g = combine_state \<Sigma>\<^sub>g" by simp
+  thus ?case by blast
+next
+  case (iter_step \<Sigma>\<^sub>c' \<Sigma>\<^sub>c'')
+  then obtain \<Sigma>\<^sub>g' where S: "\<Sigma>\<^sub>g \<leadsto>\<^sub>g \<Sigma>\<^sub>g' \<and> \<Sigma>\<^sub>c' = combine_state \<Sigma>\<^sub>g'" by fastforce
+  with iter_step have "\<Sigma>\<^sub>g' :\<^sub>g t" by fastforce
+  with iter_step S obtain \<Sigma>\<^sub>g'' where "iter (\<leadsto>\<^sub>g) \<Sigma>\<^sub>g' \<Sigma>\<^sub>g'' \<and> \<Sigma>\<^sub>c'' = combine_state \<Sigma>\<^sub>g''" by fastforce
+  with S have "iter (\<leadsto>\<^sub>g) \<Sigma>\<^sub>g \<Sigma>\<^sub>g'' \<and> \<Sigma>\<^sub>c'' = combine_state \<Sigma>\<^sub>g''" by fastforce
+  thus ?case by blast
+qed
+
+text \<open>However, there is still one slight obstacle to overcome. Our ultimate compilation process will
+use \<open>split_vars\<close>, but our theorem is defined in terms of \<open>combine_vars\<close>. Fortunately, we can use our
+inverse theorems to get the result we need.\<close>
+
+lemma iter_correctness_forward\<^sub>g [simp]: "iter (\<leadsto>\<^sub>c) (SE\<^sub>c [FReturn\<^sub>c []] [] e\<^sub>c) \<Sigma>\<^sub>c' \<Longrightarrow> [] \<turnstile>\<^sub>d e\<^sub>c : t \<Longrightarrow> 
+    \<exists>\<Sigma>\<^sub>g'. iter (\<leadsto>\<^sub>g) (SE\<^sub>g [FReturn\<^sub>g []] [] (split_vars e\<^sub>c)) \<Sigma>\<^sub>g' \<and> \<Sigma>\<^sub>c' = combine_state \<Sigma>\<^sub>g'"
+proof -
+  assume "iter (\<leadsto>\<^sub>c) (SE\<^sub>c [FReturn\<^sub>c []] [] e\<^sub>c) \<Sigma>\<^sub>c'" and T: "[] \<turnstile>\<^sub>d e\<^sub>c : t"
+  hence X: "iter (\<leadsto>\<^sub>c) (combine_state (SE\<^sub>g [FReturn\<^sub>g []] [] (split_vars e\<^sub>c))) \<Sigma>\<^sub>c'" 
+    by (simp add: split_vars_def)
+  from T have "[] \<turnstile>\<^sub>g split_vars e\<^sub>c : t" by simp
+  hence "SE\<^sub>g [FReturn\<^sub>g []] [] (split_vars e\<^sub>c) :\<^sub>g t" 
+    by (metis tcg_state_ev tcg_scons_ret tcg_snil tc\<^sub>g_nil latest_environment\<^sub>g.simps(6))
+  with X show ?thesis by simp
+qed
+
 end
